used simpler equations for sub

Syntax.v
@@ -973,10 +973,32 @@ Definition evalUniBit n1 n2 (op: UniBitOp n1 n2): word n1 -> word n2 :=
 Definition wdivN := wordBinN Nat.div.
 Definition wremN := wordBinN Nat.modulo.
 
+Definition wneg_simple sz (x: word sz) := wnot x ^+ $1.
+
+Definition wminus_simple sz (x y: word sz) := x ^+ (wneg_simple y).
+
+Lemma wneg_simple_wneg sz: forall (x: word sz), wneg_simple x = wneg x.
+Proof.
+  unfold wneg_simple.
+  intros.
+  rewrite wneg_wnot.
+  rewrite wminus_wplus_undo.
+  reflexivity.
+Qed.
+
+Lemma wminus_simple_wminus sz: forall (x y: word sz), wminus_simple x y = wminus x y.
+Proof.
+  unfold wminus_simple.
+  intros.
+  rewrite wneg_simple_wneg.
+  rewrite wminus_def.
+  reflexivity.
+Qed.
+
 Definition evalBinBit n1 n2 n3 (op: BinBitOp n1 n2 n3)
   : word n1 -> word n2 -> word n3 :=
   match op with
-    | Sub n => @wminus n
+    | Sub n => @wminus_simple n
     | Div n => @wdivN n
     | Rem n => @wremN n
     | Sll n m => (fun x y => wlshift x (wordToNat y))
